theories/cancellation/MInlineElim.v
@@ -18,23 +18,20 @@ Proof using.
      IstEq closed
     (SB.sandbox_body f) (SB.sandbox_body (inline_fsem md f))).
   { econs; ss; try refl; eauto; i.
+    { ii. destruct H0. rr. destruct x; et. exfalso.
+      exploit (wf_fns i None); [|intros []; ss].
+      rewrite lookup_fmap H1. et.
+    }
     { r. rewrite !lookup_fmap.
       destruct (Mod.fnsems md !! fn) eqn:FINDT; ss.
       destruct o; ss.
       { destruct p; ss. ii. esplits; eauto. eapply H; eauto; ss.
-        { inv H1; econs; eauto. revert wf_fns; rewrite map_Forall_lookup; intros wf_fns i x Hix;
-            specialize (wf_fns i); rewrite !lookup_fmap Hix //= in wf_fns.
-          destruct x; ss; apply wf_fns; eauto.
-        }
         hexploit (Mod.well_scoped_fns md fn (e, f)).
         { rewrite lookup_omap FINDT //. }
         i; ss; des. depdes e0; ss. des_ifs.
         { case_bool_decide; eauto. }
         { case_bool_decide; eauto. }
       }
-      intros [? ?]; rewrite map_Forall_lookup in wf_fns; hexploit (wf_fns fn None); eauto.
-      { rewrite !lookup_fmap FINDT //. }
-      intros t; inv t.
     }
   }
 
