theories/modules/Mod.v
@@ -311,26 +311,6 @@ Section ModFacts.
   Qed.
 End ModFacts.
 
-(* Tactics for map definitions. *)
-Tactic Notation "mod_tac" tactic(tac) := i;
-  let rec go :=
-    match goal with
-    | |- Sorted.StronglySorted String.le ?scopes =>
-      (apply Sorted.SSorted_nil || (apply Sorted.SSorted_cons; [go|tac]))
-    | |- map_Forall ?P (omap id ?X) => rewrite omap_insert; cbn; go
-    | |- map_Forall ?P (omap id ∅) => rewrite omap_empty; go
-    | |- map_Forall ?P (fmap ?f ?X) => rewrite fmap_insert; cbn; go
-    | |- map_Forall ?P (fmap ?f ∅) => rewrite fmap_empty; cbn; go
-    | |- map_Forall ?P ∅ => apply map_Forall_empty
-    | |- map_Forall ?P {[_:=_]} => apply map_Forall_singleton; tac
-    | |- map_Forall ?P (<[_:=_]> _) =>
-        apply map_Forall_insert_2; [tac|go]
-    | |- map_Forall ?P ?X => rewrite /X; cbn; go
-    | |- _ => set_solver
-  end in go.
-Ltac scope_solver := ss; split; i; case_decide; naive_solver.
-Tactic Notation "mod_tac" := mod_tac scope_solver.
-
 (* Lemmas related to module states and function maps *)
 Lemma dom_union_with `{Countable K} {V} (m1 m2 : gmap K (option V)) :
   dom (union_with uwnd m1 m2) =
@@ -527,6 +507,41 @@ Lemma lookup_fnsems_None `{Σ : GRA} (m1 m2 : Mod.t) (k : fname) :
   (Mod.fnsems (m1 ★ m2)) !! k = None.
 Proof. rewrite lookup_union_with => -> -> //. Qed.
 
+(* Tactics for map definitions. *)
+Tactic Notation "mod_tac1" tactic(tac) := i;
+  let rec go :=
+    match goal with
+    | |- Sorted.StronglySorted String.le ?scopes =>
+      (apply Sorted.SSorted_nil || (apply Sorted.SSorted_cons; [go|tac]))
+    | |- map_Forall ?P (omap id ?X) => rewrite omap_insert; cbn; go
+    | |- map_Forall ?P (omap id ∅) => rewrite omap_empty; go
+    | |- map_Forall ?P (fmap ?f ?X) => rewrite fmap_insert; cbn; go
+    | |- map_Forall ?P (fmap ?f ∅) => rewrite fmap_empty; cbn; go
+    | |- map_Forall ?P ∅ => apply map_Forall_empty
+    | |- map_Forall ?P {[_:=_]} => apply map_Forall_singleton; tac
+    | |- map_Forall ?P (<[_:=_]> _) =>
+        apply map_Forall_insert_2; [tac|go]
+    | |- map_Forall ?P ?X => rewrite /X; cbn; go
+    | |- _ => set_solver
+  end in go.
+Ltac scope_solver := ss; split; i; case_decide; naive_solver.
+Tactic Notation "mod_tac1" := mod_tac1 scope_solver.
+
+Tactic Notation "mod_tac" tactic(tac) :=
+  i; repeat (eapply map_Forall_union_with; [set_solver|]); esplits; mod_tac1 tac.
+Tactic Notation "mod_tac" := mod_tac scope_solver.
+
+Arguments Mod.add : simpl never.
+Arguments Mod.fnsems : simpl never.
+
+Ltac unfold_fnsem :=
+  rewrite /Mod.fnsems /=;
+  match goal with | [|-context[?x]] =>
+    match type of x with gmap fname (option (emask * (option fspec_rel * fbody))) =>
+       rewrite {1}/x /=
+    end
+  end.
+
 Hint Extern 80 (Mod.fnsems (_ ★ _) !! _ = Some _) => eapply lookup_fnsems_l2 : simpl_map.
 Hint Extern 80 (Mod.fnsems (_ ★ _) !! _ = Some _) => eapply lookup_fnsems_r2 : simpl_map.
 Hint Extern 80 (Mod.fnsems (_ ★ _) !! _ = None) => eapply lookup_fnsems_None : simpl_map.
@@ -543,14 +558,6 @@ Global Hint Extern 90 =>
       (eapply Mod.lookup_add_r;
         [eauto|eapply Mod.add_wf_inv in H as [? [? [? ?]]]]; progress simpl_map)
     end : simpl_map.
-
-Ltac unfold_fnsem :=
-  rewrite /Mod.fnsems /=;
-  match goal with | [|-context[?x]] =>
-    match type of x with gmap fname (option (emask * (option fspec_rel * fbody))) =>
-       rewrite {1}/x /=
-    end
-  end.
 Hint Extern 81 (Mod.fnsems _ !! _ = Some _) => unfold_fnsem; simpl_map; eauto : simpl_map.
 Hint Extern 81 (Mod.fnsems _ !! _ = None) => unfold_fnsem; simpl_map; eauto : simpl_map.
 Arguments Mod.add : simpl never.
