theories/simulations/msim/TacticsInit.v
@@ -10,35 +10,20 @@ Ltac init_sim :=
       | (refl||eauto using submseteq_nil_l)
       | (refl||eauto using submseteq_nil_l)
       | try set_solver
+      | mod_tac
       |]
     | econs; intros Hwf;
       [ (refl||eauto using submseteq_nil_l)
+      | mod_tac
       |
       | intros fn; eapply ISim.sim_fun_strong; intros Hfn; set_unfold in Hfn; des; subst
       ]
     ]).
 
 Ltac init_simF :=
+  let wfs := fresh "WFS" in
   let wft := fresh "WFT" in
-  (tryif (
-    rewrite /ISim.sim_fun; simpl_map; intros wft; eexists; split; first refl
-  )
-  then idtac
-  else (
-    match goal with
-    | |- ISim.sim_fun _ ?ms ?mt _ _ =>
-      intros wft;
-      let wfs := fresh "WFS" in
-      assert (wfs : Mod.wf ms);
-        [eapply Mod.add_wf_inv in wft as [? [? [? ?]]];
-        apply Mod.add_wf;
-          [ econs; [mod_tac | (done || prove_nodup)]
-          | ss
-          | try set_solver
-          | (ss || prove_nodup) ]
-        | ]
-    end; simpl_map; eexists; split; first refl
-  ));
+  rewrite /ISim.sim_fun; intros wfs wft; simpl_map; eexists; split; first refl;
   iIntros (arg st_src st_tgt) "IST"; iApply wsim_isim;
   rewrite /SB.sandbox_body; simpl fst; simpl snd.
 
